End of empire ...

theories/tests/spawn.v
@@ -3,15 +3,38 @@ From iris_c.clang.lib Require Import lock.
 From iris_c.lib Require Import int.
 
 Section test.
-  Context `{clangG Σ}.
+  Context `{clangG Σ, lockG Σ} (N: namespace) (γ: gname).
 
-  Definition x : ident := 1.
-  Definition r : ident := 2.
-  Definition l : ident.
+  Variable lx : addr.
+  Variable l : val.
+  Definition f_acquire : ident := 3.
+  Definition f_release : ident := 4.
+
+  Definition R: iProp Σ := (∃ vx: int32, lx ↦ vx @ Tint32)%I.
   
   Definition add: expr :=
-    lock l
-    r <- vtrue.
+    Ecall Tvoid f_acquire [Evalue l] ;;
+    lx <- !lx@Tint32 + 1;;
+    Ecall Tvoid f_release [Evalue l].
 
-  Lemma add_spec:
-    r ↦ 
+  Lemma add_safe (lr: addr) ks:
+    own_stack ks ∗ is_lock N γ l R ∗
+    text_interp f_release (Function Tvoid [(x, tylock)] release) ∗
+    text_interp f_acquire (Function Tvoid [(x, tylock)] acquire)
+    ⊢ WP add {{ _, True }}.
+  Proof.
+    iIntros "(Hs & #Hlk & H1 & H2)". unfold add.
+    wp_unfill (Ecall _ _ _).
+    iApply acquire_spec. iFrame. iFrame "#".
+    iIntros "Hlked HR Hks".
+    iDestruct "HR" as (?) "Hvx".
+    wp_skip. wp_load. wp_op. wp_assign.
+    iApply (release_spec []). iFrame "Hlk".
+    iFrame. iSplitL "Hvx"; first by iExists _.
+    iIntros "Hks". iApply wp_value=>//.
+  Qed.
+
+  (* It is just DRF property -- though we can have a stronger spec
+     by encoding some receipt tokens *)
+
+  
